progress.md
@@ -7,7 +7,7 @@
 
 ## prelude
 
-- session_prelude.v (1085 lines) [v]
+- session_prelude.v (1164 lines) [v]
 - definitions.v (314 lines) [v]
 - coq_session.v (646 lines) [v]
 
@@ -15,7 +15,7 @@
 
 1. versionVector.v (567 lines) [v]
 2. sort.v (198 lines) [v]
-3. gossip.v [x] (WIP)
+3. gossip.v (618 lines) [v]
 4. processRequest.v [x]
 5. coq_session_client.v (808 lines) [v]
 6. nat_equivalence.v [x]
